

## Examples

**De Morgan:**  $\neg(p \wedge q) \vdash (\neg p \vee \neg q)$

Proof (dynamic-single mode):

1	$\neg(p \wedge q)$	
2	$\neg(\neg p \vee \neg q)$	
3	$\neg p$	
4	$(\neg p \vee \neg q)$	$\vee I \quad 3$
5	$\perp$	$\perp I \quad 2, 4$
6	$\neg\neg p$	$\neg I \quad 3 - 5$
7	$p$	$\neg E \quad 6$
8	$\neg q$	
9	$(\neg p \vee \neg q)$	$\vee I \quad 8$
10	$\perp$	$\perp I \quad 2, 9$
11	$\neg\neg q$	$\neg I \quad 8 - 10$
12	$q$	$\neg E \quad 11$
13	$(p \wedge q)$	$\wedge I \quad 7, 12$
14	$\perp$	$\perp I \quad 1, 13$
15	$\neg\neg(\neg p \vee \neg q)$	$\neg I \quad 2, 14$
16	$(\neg p \vee \neg q)$	$\neg E \quad 15$

**Excluded Middle:**  $\vdash (p \vee \neg p)$

Proof (fixed mode to 60pt):

1	$\neg(p \vee \neg p)$	
2	$p$	
3	$(p \vee \neg p)$	$\vee I \quad 2$
4	$\perp$	$\perp I \quad 1, 3$
5	$\neg p$	$\neg I \quad 2 - 4$
6	$(p \vee \neg p)$	$\vee I \quad 5$
7	$\perp$	$\perp I \quad 1, 6$
8	$\neg\neg(p \vee \neg p)$	$\neg I \quad 1 - 7$
9	$p \vee \neg p$	$\neg E \quad 8$

**Non-Contradiction:**  $\vdash \neg(p \wedge \neg p)$

Proof (fixed mode to the default 2.5em):

1	$(p \wedge \neg p)$	
2	$p$	$\wedge E \quad 1$
3	$\neg p$	$\wedge E \quad 2$
4	$\perp$	$\perp I \quad 1, 2$
5	$\neg(p \wedge \neg p)$	$\neg I \quad 1 - 4$

## Some Natural Deduction Rules

$m$	$p$
$n$	$q$
$o$	$(p \wedge q) \quad \wedge I \quad m, n$

$m$	$(p \wedge q)$
$n_1$	$p \quad \wedge E \quad m$
$n_2$	$q \quad \wedge E \quad m$

$m$	$p$
$n$	$(p \vee q) \quad \vee I \quad m$

$a$	$(p \vee q)$
$b$	$p$
$c$	$r$
$d$	$q$
$e$	$r$
$f$	$r \quad \vee E \quad a, b - c, d - e$